

4.18. MATRICES

Let us consider a set of simultaneous equations,

$$x + 2y + 3z + 5t = 0$$

$$4x + 2y + 5z + 7t = 0$$

$$3x + 4y + 2z + 6t = 0.$$

Now we write down the coefficients of x, y, z, t of the above equations and enclose them within brackets and then we get

$$A = \begin{bmatrix} 1 & 2 & 3 & 5 \\ 4 & 2 & 5 & 7 \\ 3 & 4 & 2 & 6 \end{bmatrix}$$

The above system of numbers, arranged in a rectangular array in rows and columns and bounded by the brackets, is called a matrix.

It has got 3 rows and 4 columns and in all $3 \times 4 = 12$ elements. It is termed as 3×4 matrix, to be read as [3 by 4 matrix]. In the double subscripts of an element, the first subscript determines the row and the second subscript determines the column in which the element lies, a_{ij} lies in the i th row and j th column.

4.19 VARIOUS TYPES OF MATRICES

(a) **Row Matrix.** If a matrix has only one row and any number of columns, it is called a Row matrix, e.g.,

$$[2 \ 7 \ 3 \ 9]$$

(b) **Column Matrix.** A matrix, having one column and any number of rows, is called a Column matrix, e.g.,

$$\begin{bmatrix} 1 \\ 2 \\ 3 \end{bmatrix}$$

(c) **Null Matrix or Zero Matrix.** Any matrix, in which all the elements are zeros, is called a Zero matrix or Null matrix e.g.,

$$\begin{bmatrix} 0 & 0 & 0 & 0 \\ 0 & 0 & 0 & 0 \end{bmatrix}$$

(d) **Square Matrix.** A matrix, in which the number of rows is equal to the number of columns, is called a square matrix e.g.,

$$\begin{bmatrix} 2 & 5 \\ 1 & 4 \end{bmatrix}$$

(e) **Diagonal Matrix.** A square matrix is called a diagonal matrix, if all its non-diagonal elements are zero e.g.,

$$\begin{bmatrix} 1 & 0 & 0 \\ 0 & 3 & 0 \\ 0 & 0 & 4 \end{bmatrix}$$

(f) **Unit or Identity Matrix.** A square matrix is called a unit matrix if all the diagonal elements are unity and non-diagonal elements are zero e.g.,

$$\begin{bmatrix} 1 & 0 & 0 \\ 0 & 1 & 0 \\ 0 & 0 & 1 \end{bmatrix}, \begin{bmatrix} 1 & 0 \\ 0 & 1 \end{bmatrix}$$

(g) **Symmetric Matrix.** A square matrix will be called symmetric, if for all values of i and j , i.e. $a_{ij} = a_{ji}$ or $A' = A$ e.g.,

$$\begin{bmatrix} a & h & g \\ h & b & f \\ g & f & c \end{bmatrix}$$

(h) **Skew Symmetric Matrix.** A square matrix is called skew symmetric matrix, if

(1) $a_{ij} = -a_{ji}$ for all values of i and j , or $A' = -A$

(2) All diagonal elements are zero, e.g.,

$$\begin{bmatrix} 0 & -h & -g \\ h & 0 & -f \\ g & f & 0 \end{bmatrix}$$

(i) **Triangular Matrix (Echelon form).** A square matrix, all of whose elements below the leading diagonal are zero, is called an upper triangular matrix. A square matrix, all of whose elements above the leading diagonal are zero, is called a lower triangular matrix e.g.,

$$\begin{bmatrix} 1 & 3 & 2 \\ 0 & 4 & 1 \\ 0 & 0 & 6 \end{bmatrix}$$

$$\begin{bmatrix} 2 & 0 & 0 \\ 4 & 1 & 0 \\ 5 & 6 & 7 \end{bmatrix}$$

Upper triangular matrix

Lower triangular matrix

(j) **Transpose of a Matrix.** If in a given matrix A , we interchange the rows and the corresponding columns, the new matrix obtained is called the transpose of the matrix A and is denoted by A' or A^T e.g.,

$$A = \begin{bmatrix} 2 & 3 & 4 \\ 1 & 0 & 5 \\ 6 & 7 & 8 \end{bmatrix}, A' = \begin{bmatrix} 2 & 1 & 6 \\ 3 & 0 & 7 \\ 4 & 5 & 8 \end{bmatrix}$$

(k) **Orthogonal Matrix.** A square matrix A is called an orthogonal matrix if the product of the matrix A and the transpose matrix A' is an identity matrix e.g.,

$$A \cdot A' = I$$

if $|A| = 1$, matrix A is proper.

(l) **Conjugate of a Matrix.**

Let $A = \begin{bmatrix} 1+i & 2-3i & 4 \\ 7+2i & -i & 3-2i \end{bmatrix}$

Conjugate of matrix A is \bar{A}

$$\bar{A} = \begin{bmatrix} 1-i & 2+3i & 4 \\ 7-2i & i & 3+2i \end{bmatrix}$$

(m) **Matrix A^0 .** Transpose of the conjugate of a matrix A is denoted by A^0 .

Let

$$A = \begin{bmatrix} 1+i & 2-3i & 4 \\ 7+2i & -i & 3-2i \\ 1-i & 2+3i & 4 \\ 7-2i & +i & 3+2i \end{bmatrix}$$

$$\bar{A} = \begin{bmatrix} 1-i & 7-2i \\ 2+3i & i \\ 4 & 3+2i \end{bmatrix}$$

$$A^0 = \begin{bmatrix} 1-i & 7-2i \\ 2+3i & i \\ 4 & 3+2i \end{bmatrix}$$

or

(n) **Unitary Matrix.** A square matrix A is said to be unitary if

$$A^0 A = I$$

e.g. $A = \begin{bmatrix} \frac{1+i}{2} & \frac{-1+i}{2} \\ \frac{1+i}{2} & \frac{1-i}{2} \end{bmatrix}, A^0 = \begin{bmatrix} \frac{1-i}{2} & \frac{1-i}{2} \\ \frac{-1-i}{2} & \frac{1+i}{2} \end{bmatrix}, A \cdot A^0 = I$

(o) **Hermitian Matrix.** A square matrix $A = (a_{ij})$ is called **Hermitian matrix**, if every i -jth element of A is equal to conjugate complex j -ith element of A .

In other words

$$a_{ij} = \bar{a}_{ji}$$

e.g. $\begin{bmatrix} 1 & 2+3i & 3+i \\ 2-3i & 2 & 1-2i \\ 3-i & 1+2i & 5 \end{bmatrix}$

Necessary and sufficient condition for a matrix A to be Hermitian is that $A = A^0$ i.e. conjugate transpose of A

or

$$A = (\bar{A})'$$

(p) **Skew Hermitian Matrix.** A square matrix $A = (a_{ij})$ will be called a Skew Hermitian matrix if every i -jth element of A is equal to negative conjugate complex of j -ith element of A .

In other words

$$a_{ij} = -\bar{a}_{ji}$$

All the elements in the principal diagonal will be of the form

$$a_{ii} = -\bar{a}_{ii} \text{ or } a_{ii} + \bar{a}_{ii} = 0$$

If

$$a_{ii} = a + ib \text{ then } \bar{a}_{ii} = a - ib$$

$$(a + ib) + (a - ib) = 0 \text{ or } 2a = 0 \text{ or } a = 0$$

So a_{ii} is pure imaginary or $a_{ii} = 0$

Hence all the diagonal elements of a Skew Hermitian Matrix are either zeros or pure imaginary.

e.g.

$$\begin{bmatrix} i & 2-3i & 4+5i \\ -(2+3i) & 0 & 2i \\ -(4-5i) & 2i & -3i \end{bmatrix}$$

The necessary and sufficient condition for a matrix A to be Skew Hermitian is that

$$A^0 = -A$$

$$(\bar{A})' = -A$$

(q) **Idempotent Matrix.** A matrix such that $A^2 = A$ is called Idempotent Matrix.

e.g. $A = \begin{bmatrix} 2 & -2 & -4 \\ -1 & 3 & 4 \\ 1 & -2 & -3 \end{bmatrix}, A^2 = \begin{bmatrix} 2 & -2 & -4 \\ -1 & 3 & 4 \\ 1 & -2 & -3 \end{bmatrix} \begin{bmatrix} 2 & -2 & -4 \\ -1 & 3 & 4 \\ 1 & -2 & -3 \end{bmatrix} = \begin{bmatrix} 2 & -2 & -4 \\ -1 & 3 & 4 \\ 1 & -2 & -3 \end{bmatrix} = A$

(r) **Periodic Matrix.** A matrix A will be called a Periodic Matrix, if

$$A^{k+1} = A$$

where k is a +ve integer. If k is the least +ve integer, for which $A^{k+1} = A$, then k is said to be the period of A . If we choose $k = 1$ we get $A^2 = A$ and we call it to be idempotent matrix.

(s) **Nilpotent Matrix.** A matrix will be called a Nilpotent matrix, if $A^k = 0$ (null matrix) where k is a +ve integer; if however k is the least +ve integer for which $A^k = 0$, then k is the index of the nilpotent matrix.

e.g. $A = \begin{bmatrix} ab & b^2 \\ -a^2 & -ab \end{bmatrix}, A^2 = \begin{bmatrix} ab & b^2 \\ -a^2 & -ab \end{bmatrix} \begin{bmatrix} ab & b^2 \\ -a^2 & -ab \end{bmatrix} = \begin{bmatrix} 0 & 0 \\ 0 & 0 \end{bmatrix} = 0$

A is nilpotent matrix whose index is 2.

(t) **Involuntary Matrix.** A matrix A will be called an Involuntary matrix, if $A^2 = I$ (unit matrix). Since $I^2 = I$ always. Unit matrix is involuntary.

(u) **Equal Matrices.** Two matrices are said to be equal if

(i) They are of the same order.

(ii) The elements in the corresponding positions are equal.

Thus if

$$A = \begin{bmatrix} 2 & 3 \\ 1 & 4 \end{bmatrix}, B = \begin{bmatrix} 2 & 3 \\ 1 & 4 \end{bmatrix}$$

Here

$$A = B$$

(v) **Singular Matrix :** If the determinant of the matrix is zero, then the matrix is known as singular matrix. e.g. If $|A| = \begin{vmatrix} 1 & 2 \\ 3 & 6 \end{vmatrix} = 6 - 6 = 0$, then A is a singular matrix.

Example 1. Find the values of x, y, z and ' a ' which satisfy the matrix equation.

$$\begin{bmatrix} x+3 & 2y+x \\ z-1 & 4a-6 \end{bmatrix} = \begin{bmatrix} 0 & -7 \\ 3 & 2a \end{bmatrix}$$

Solution. As the given matrices are equal, so their corresponding elements are equal.

$$x+3 = 0 \text{ or } x = -3 \quad \dots(1)$$

$$2y+x = -7 \quad \dots(2)$$

$$z-1 = 3 \text{ or } z = 4 \quad \dots(3)$$

$$4a-6 = 2a \text{ or } a = 3 \quad \dots(4)$$

Putting the value of $x = -3$ from (1) into (2), we have

$$2y-3 = -7 \text{ or } y = -2$$

$$x = -3, y = -2, z = 4, a = 3$$

Ans.

20 ADDITION OF MATRICES

If A and B be two matrices of the same order, then their sum, $A+B$ is defined as the matrix, each element of which is the sum of the corresponding elements of A and B .

Thus if

$$A = \begin{bmatrix} 4 & 2 & 5 \\ 1 & 3 & -6 \end{bmatrix}, B = \begin{bmatrix} 1 & 0 & 2 \\ 3 & 1 & 4 \end{bmatrix}$$

$$A+B = \begin{bmatrix} 4+1 & 2+0 & 5+2 \\ 1+3 & 3+1 & -6+4 \end{bmatrix} = \begin{bmatrix} 5 & 2 & 7 \\ 4 & 4 & -2 \end{bmatrix}$$

If

$$A = [a_{ij}], B = [b_{ij}] \text{ then } A + B = [a_{ij} + b_{ij}]$$

Example 2. Show that any square matrix can be expressed as the sum of two matrices, one symmetric and the other anti-symmetric.

Solution. Let A be a given square matrix.

Then

$$A = \frac{1}{2}(A + A') + \frac{1}{2}(A - A')$$

Now

$$(A + A')' = A' + A = A + A'$$

$\therefore A + A'$ is a symmetric matrix.

Also

$$(A - A')' = A' - A = -(A - A')$$

$\therefore A - A'$ or $\frac{1}{2}(A - A')$ is an anti-symmetric matrix.

$$A = \frac{1}{2}(A + A') + \frac{1}{2}(A - A')$$

= Symmetric matrix + antisymmetric matrix

Proved.

Example 3. Write matrix (A) given below as the sum of a symmetric and a skew symmetric matrix.

$$A = \begin{bmatrix} 1 & 2 & 4 \\ -2 & 5 & 3 \\ -1 & 6 & 3 \end{bmatrix}$$

Solution: $A = \begin{bmatrix} 1 & 2 & 4 \\ -2 & 5 & 3 \\ -1 & 6 & 3 \end{bmatrix}$ On transposing we get $A' = \begin{bmatrix} 1 & -2 & -1 \\ 2 & 5 & 6 \\ 4 & 3 & 3 \end{bmatrix}$

On adding A and A' , we have

$$A + A' = \begin{bmatrix} 1 & 2 & 4 \\ -2 & 5 & 3 \\ -1 & 6 & 3 \end{bmatrix} + \begin{bmatrix} 1 & -2 & -1 \\ 2 & 5 & 6 \\ 4 & 3 & 3 \end{bmatrix} = \begin{bmatrix} 2 & 0 & 3 \\ 0 & 10 & 9 \\ 3 & 9 & 6 \end{bmatrix} \quad \dots(1)$$

On subtracting A' from A we get

$$A - A' = \begin{bmatrix} 1 & 2 & 4 \\ -2 & 5 & 3 \\ -1 & 6 & 3 \end{bmatrix} - \begin{bmatrix} 1 & -2 & -1 \\ 2 & 5 & 6 \\ 4 & 3 & 3 \end{bmatrix} = \begin{bmatrix} 0 & 4 & 5 \\ -4 & 0 & -3 \\ -5 & 3 & 0 \end{bmatrix} \quad \dots(2)$$

On adding (1) and (2), we have

$$2A = \begin{bmatrix} 2 & 0 & 3 \\ 0 & 10 & 9 \\ 3 & 9 & 6 \end{bmatrix} + \begin{bmatrix} 0 & 4 & 5 \\ -4 & 0 & -3 \\ -5 & 3 & 0 \end{bmatrix}$$

$$A = \begin{bmatrix} 1 & 0 & \frac{3}{2} \\ 0 & 5 & \frac{9}{2} \\ \frac{3}{2} & \frac{9}{2} & 3 \end{bmatrix} + \begin{bmatrix} 0 & 2 & \frac{5}{2} \\ -2 & 0 & -\frac{3}{2} \\ -\frac{5}{2} & \frac{3}{2} & 0 \end{bmatrix}$$

= [Symmetric matrix] + [Skew symmetric matrix.] **Ans.**

4. If $A = \begin{bmatrix} 0 & 2 & 0 \\ 1 & 0 & 3 \\ 1 & 1 & 2 \end{bmatrix}$, $B = \begin{bmatrix} 1 & 2 & 1 \\ 2 & 1 & 0 \\ 0 & 0 & 3 \end{bmatrix}$
Find (i) $2A + 3B$ (ii) $3A - 4B$.

Ans. (i) $\begin{bmatrix} 3 & 10 & 3 \\ 8 & 3 & 6 \\ 2 & 2 & 13 \end{bmatrix}$, (ii) $\begin{bmatrix} -4 & -2 & -4 \\ -5 & -4 & 9 \\ 3 & 3 & -6 \end{bmatrix}$

5. If A is a skew-symmetric matrix of odd order, then the determinant of A is

- (a) -1. (b) 0. (c) 1. (d) a real number.

Ans. (b)

6. Let A be a non-singular matrix. Then the inverse of the matrix AA^T

- (a) is symmetric (b) is skew-symmetric (c) does not exist (d) equals $A^{-1}(A^{-1})^T$

(A.M.I.E.T.E., Summer 2003) **Ans.** (a)

4.24. MULTIPLICATION

The product of two matrices A and B is only possible if the number of columns in A is equal to the number of rows in B .

Let $A = [a_{ij}]$ be an $m \times n$ matrix and $B = [b_{ij}]$ be an $n \times p$ matrix. Then the product AB of these matrices is an $m \times p$ matrix $C = [c_{ij}]$ where

$$c_{ij} = a_{i1}b_{1j} + a_{i2}b_{2j} + a_{i3}b_{3j} + \dots + a_{in}b_{nj}$$

4.25. $(AB)' = B'A'$

If A and B are two matrices conformal for product AB , then show that $(AB)' = B'A'$, where dash represents transpose of a matrix.

Solution. Let $A = [a_{ij}]$ be an $m \times n$ matrix and $B = [b_{ij}]$ be $n \times p$ matrix.

Since AB is an $m \times p$ matrix, $(AB)'$ is a $p \times m$ matrix.

Further B' is $p \times n$ matrix and A' an $n \times m$ matrix and therefore $B'A'$ is a $p \times m$ matrix.

Thus $(AB)'$ and $B'A'$ are matrices of the same order.

Now the (j, i) th element of $(AB)' = (i, j)$ th element of $(AB) = \sum_{k=1}^n a_{ik}b_{kj} \dots(1)$

Also the j th row of B' is $b_{1j}, b_{2j}, \dots, b_{nj}$ and i th column of A' is $a_{i1}, a_{i2}, a_{i3}, \dots, a_{in}$.

$\therefore (j, i)$ th element of $B'A' = \sum_{k=1}^n b_{kj}a_{ik} \dots(2)$

From (1) and (2) we have (j, i) th element of $(AB)' = (j, i)$ th element of $B'A'$.

As the matrices $(AB)'$ and $B'A'$ are of the same order and their corresponding elements are equal, we have $(AB)' = B'A'$.

Proved

4.26. PROPERTIES OF MATRIX MULTIPLICATION

1. Multiplication of matrices is not commutative.

$$AB \neq BA$$

2. Matrix multiplication is associative, if confirmability is assured.

$$A(BC) = (AB)C$$

3. Matrix multiplication is distributive with respect to addition.

$$A(B+C) = AB+AC$$

4. Multiplication of matrix A by unit matrix.

$$AI = IA = A$$

5. Multiplicative inverse of a matrix exists if $|A| \neq 0$.

$$A \cdot A^{-1} = A^{-1} \cdot A = I$$

The product $= \begin{bmatrix} 0 & 0 \\ 0 & 0 \end{bmatrix} = 0$.

Proved.

Example 15. Verify that

$$A = \frac{1}{3} \begin{bmatrix} 1 & 2 & 2 \\ 2 & 1 & -2 \\ -2 & 2 & -1 \end{bmatrix} \text{ is orthogonal.}$$

Solution.

$$A = \frac{1}{3} \begin{bmatrix} 1 & 2 & 2 \\ 2 & 1 & -2 \\ -2 & 2 & -1 \end{bmatrix} \therefore A' = \frac{1}{3} \begin{bmatrix} 1 & 2 & -2 \\ 2 & 1 & 2 \\ 2 & -2 & -1 \end{bmatrix}$$

$$AA' = \frac{1}{9} \begin{bmatrix} 1 & 2 & 2 \\ 2 & 1 & -2 \\ -2 & 2 & -1 \end{bmatrix} \begin{bmatrix} 1 & 2 & -2 \\ 2 & 1 & 2 \\ 2 & -2 & -1 \end{bmatrix}$$

$$= \frac{1}{9} \begin{bmatrix} 9 & 0 & 0 \\ 0 & 9 & 0 \\ 0 & 0 & 9 \end{bmatrix} = \begin{bmatrix} 1 & 0 & 0 \\ 0 & 1 & 0 \\ 0 & 0 & 1 \end{bmatrix} = I$$

Hence A is an orthogonal matrix. Verified.

Example 16. Determine the values of α, β, γ when

$$\begin{bmatrix} 0 & 2\beta & \gamma \\ \alpha & \beta & -\gamma \\ \alpha & -\beta & \gamma \end{bmatrix} \text{ is orthogonal.}$$

Solution.

$$\text{Let } A = \begin{bmatrix} 0 & 2\beta & \gamma \\ \alpha & \beta & -\gamma \\ \alpha & -\beta & \gamma \end{bmatrix}$$

On transposing A, we have

$$A' = \begin{bmatrix} 0 & \alpha & \alpha \\ 2\beta & \beta & -\beta \\ \gamma & -\gamma & \gamma \end{bmatrix}$$

If A is orthogonal, then $AA' = I$

$$\begin{bmatrix} 0 & 2\beta & \gamma \\ \alpha & \beta & -\gamma \\ \alpha & -\beta & \gamma \end{bmatrix} \begin{bmatrix} 0 & \alpha & \alpha \\ 2\beta & \beta & -\beta \\ \gamma & -\gamma & \gamma \end{bmatrix} = \begin{bmatrix} 1 & 0 & 0 \\ 0 & 1 & 0 \\ 0 & 0 & 1 \end{bmatrix}$$

$$\begin{bmatrix} 4\beta^2 + \gamma^2 & 2\beta^2 - \gamma^2 & -2\beta^2 + \gamma^2 \\ 2\beta^2 - \gamma^2 & \alpha^2 + \beta^2 + \gamma^2 & \alpha^2 - \beta^2 - \gamma^2 \\ -2\beta^2 + \gamma^2 & \alpha^2 - \beta^2 - \gamma^2 & \alpha^2 + \beta^2 + \gamma^2 \end{bmatrix} = \begin{bmatrix} 1 & 0 & 0 \\ 0 & 1 & 0 \\ 0 & 0 & 1 \end{bmatrix}$$

Equating the corresponding elements, we have

$$\begin{cases} 4\beta^2 + \gamma^2 = 1 \\ 2\beta^2 - \gamma^2 = 0 \end{cases} \Rightarrow \beta = \pm \frac{1}{\sqrt{6}}, \gamma = \pm \frac{1}{\sqrt{3}}$$

$$\alpha^2 + \beta^2 + \gamma^2 = 1 \text{ as } \beta = \pm \frac{1}{\sqrt{6}}, \gamma = \pm \frac{1}{\sqrt{3}}, \alpha = \pm \frac{1}{\sqrt{2}} \text{ Ans.}$$

$$\text{where } A_1 = \begin{vmatrix} b_2 & b_3 \\ c_2 & c_3 \end{vmatrix} = b_2c_3 - b_3c_2, \quad A_2 = -\begin{vmatrix} b_1 & b_3 \\ c_1 & c_3 \end{vmatrix} = -b_1c_3 + b_3c_1$$

$$A_3 = \begin{vmatrix} b_1 & b_2 \\ c_1 & c_2 \end{vmatrix} = b_1c_2 - b_2c_1, \quad B_1 = -\begin{vmatrix} a_2 & a_3 \\ c_2 & c_3 \end{vmatrix} = -a_2c_3 + a_3c_2$$

$$B_2 = \begin{vmatrix} a_1 & a_3 \\ c_1 & c_3 \end{vmatrix} = a_1c_3 - a_3c_1, \quad B_3 = -\begin{vmatrix} a_1 & a_2 \\ c_1 & c_2 \end{vmatrix} = -a_1c_2 + a_2c_1$$

$$C_1 = \begin{vmatrix} a_2 & a_3 \\ b_2 & b_3 \end{vmatrix} = a_2b_3 - a_3b_2, \quad C_2 = -\begin{vmatrix} a_1 & a_3 \\ b_1 & b_3 \end{vmatrix} = -a_1b_3 + a_3b_1$$

$$C_3 = \begin{vmatrix} a_1 & a_2 \\ b_1 & b_2 \end{vmatrix} = a_1b_2 - a_2b_1$$

Then the transpose of the matrix of co-factors

$$\begin{bmatrix} A_1 & B_1 & C_1 \\ A_2 & B_2 & C_2 \\ A_3 & B_3 & C_3 \end{bmatrix}$$

is called the adjoint of the matrix A and is written as $\text{adj } A$.

4.28 PROPERTY OF ADJOINT MATRIX

The product of a matrix A and its adjoint is equal to unit matrix multiplied by the determinant

If A be a square matrix, then $(\text{Adjoint } A) \cdot A = A \cdot (\text{Adjoint } A) = |A| \cdot I$

$$\text{Let } A = \begin{bmatrix} a_1 & a_2 & a_3 \\ b_1 & b_2 & b_3 \\ c_1 & c_2 & c_3 \end{bmatrix} \text{ and } \text{adj. } A = \begin{bmatrix} A_1 & B_1 & C_1 \\ A_2 & B_2 & C_2 \\ A_3 & B_3 & C_3 \end{bmatrix}$$

$$A \cdot (\text{adj. } A) = \begin{bmatrix} a_1 & a_2 & a_3 \\ b_1 & b_2 & b_3 \\ c_1 & c_2 & c_3 \end{bmatrix} \times \begin{bmatrix} A_1 & B_1 & C_1 \\ A_2 & B_2 & C_2 \\ A_3 & B_3 & C_3 \end{bmatrix}$$

$$= \begin{bmatrix} a_1A_1 + a_2A_2 + a_3A_3 & a_1B_1 + a_2B_2 + a_3B_3 & a_1C_1 + a_2C_2 + a_3C_3 \\ b_1A_1 + b_2A_2 + b_3A_3 & b_1B_1 + b_2B_2 + b_3B_3 & b_1C_1 + b_2C_2 + b_3C_3 \\ c_1A_1 + c_2A_2 + c_3A_3 & c_1B_1 + c_2B_2 + c_3B_3 & c_1C_1 + c_2C_2 + c_3C_3 \end{bmatrix}$$

$$\begin{bmatrix} |A| & 0 & 0 \\ 0 & |A| & 0 \\ 0 & 0 & |A| \end{bmatrix} = |A| \begin{bmatrix} 1 & 0 & 0 \\ 0 & 1 & 0 \\ 0 & 0 & 1 \end{bmatrix} = |A| I$$

4.29 INVERSE OF A MATRIX

If A and B are two square matrices of the same order, such that

$$AB = BA = I$$

then B is called the inverse of A i.e. $B = A^{-1}$ and A is the inverse of B.

Condition for a square matrix A to possess an inverse is that matrix A is non-singular, i.e., $|A| \neq 0$

If A is a square matrix and B be its inverse, then $AB = I$

Taking determinant of both sides

$$|AB| = |I| \text{ or } |A||B| = 1$$

(A.M.I.E. Summer 2004)

(I = unit matrix)

From this relation it is clear that $|A| \neq 0$

the matrix A is non-singular.

to find the inverse matrix with the help of adjoint matrix

We know that $A \cdot (\text{Adj. } A) = |A| I$

$$A \cdot (\text{Adj. } A) \cdot \frac{1}{|A|} = I \quad \text{Provided } |A| \neq 0$$

$$A \cdot A^{-1} = I \quad \therefore A^{-1} = \frac{1}{|A|} (\text{Adj. } A)$$

Example 18. If $A = \begin{bmatrix} 3 & -3 & 4 \\ 2 & -3 & 4 \\ 0 & -1 & 1 \end{bmatrix}$, find A^{-1} . (A.M.I.E. Summer 2004)

$$\text{Solution. } A = \begin{bmatrix} 3 & -3 & 4 \\ 2 & -3 & 4 \\ 0 & -1 & 1 \end{bmatrix}$$

$$|A| = 3(-3+4) + 3(2-0) + 4(-2-0) = 3+6-8 = 1$$

The co-factors of elements of various rows of $|A|$ are

$$\begin{bmatrix} (-3+4) & (-2-0) & (-2-0) \\ (3-4) & (3-0) & (3-0) \\ (-12+12) & (-12+8) & (-9+6) \end{bmatrix}$$

Therefore the matrix formed by the co-factors of $|A|$ is

$$\begin{bmatrix} 1 & -2 & -2 \\ -1 & 3 & 3 \\ 0 & -4 & -3 \end{bmatrix}, \text{Adj. } A = \begin{bmatrix} 1 & -1 & 0 \\ -2 & 3 & -4 \\ -2 & 3 & -3 \end{bmatrix}$$

$$A^{-1} = \frac{1}{|A|} \text{Adj. } A = \frac{1}{1} \begin{bmatrix} 1 & -1 & 0 \\ -2 & 3 & -4 \\ -2 & 3 & -3 \end{bmatrix} = \begin{bmatrix} 1 & -1 & 0 \\ -2 & 3 & -4 \\ -2 & 3 & -3 \end{bmatrix} \quad \text{Ans.}$$

Example 19. If $A = \frac{1}{9} \begin{bmatrix} -8 & 1 & 4 \\ 4 & 4 & 7 \\ 1 & -8 & 4 \end{bmatrix}$, prove that $A^{-1} = A'$, A' being the transpose of A . (A.M.I.E., Winter 2000)

Solution. If

$$A = \frac{1}{9} \begin{bmatrix} -8 & 1 & 4 \\ 4 & 4 & 7 \\ 1 & -8 & 4 \end{bmatrix}, \quad A' = \frac{1}{9} \begin{bmatrix} -8 & 4 & 1 \\ 1 & 4 & -8 \\ 4 & 7 & 4 \end{bmatrix}$$

$$\begin{aligned} AA' &= \frac{1}{9} \begin{bmatrix} -8 & 1 & 4 \\ 4 & 4 & 7 \\ 1 & -8 & 4 \end{bmatrix} \cdot \frac{1}{9} \begin{bmatrix} -8 & 4 & 1 \\ 1 & 4 & -8 \\ 4 & 7 & 4 \end{bmatrix} \\ &= \frac{1}{81} \begin{bmatrix} 64+1+16 & -32+4+28 & -8-8+16 \\ -32+4+28 & 16+16+49 & 4-32+28 \\ -8-8+16 & 4-32+28 & 1+64+16 \end{bmatrix} \\ &= \frac{1}{81} \begin{bmatrix} 81 & 0 & 0 \\ 0 & 81 & 0 \\ 0 & 0 & 81 \end{bmatrix} = \begin{bmatrix} 1 & 0 & 0 \\ 0 & 1 & 0 \\ 0 & 0 & 1 \end{bmatrix} \quad \text{or } AA' = I \\ A' &= A^{-1} \quad \text{Proved} \end{aligned}$$

Example 20. If a matrix A satisfies a relation $A^2 + A - I = 0$ prove that A^{-1} exists and that $A^{-1} = I + A$. I being an identity matrix. (AMIE Winter 2003)

Solution. Here $A^2 + A - I = 0$ or $A^2 + A = I$ or $A(A + I) = I$

$$|A| |A + I| = |I|$$

$$|A| \neq 0 \text{ and so } A^{-1} \text{ exists.}$$

$$\text{Again } A^2 + A - I = 0 \text{ or } A^2 + A = I$$

Multiplying (1) by A^{-1} , we get

$$A^{-1}(A^2 + A) = A^{-1}I \text{ or } A + I = A^{-1}$$

$$A^{-1} = I + A$$

Proved

Example 21. If A and B are non-singular matrices of the same order then,

$$(AB)^{-1} = B^{-1} \cdot A^{-1}$$

Hence, prove that $(A^{-1})^m = (A^m)^{-1}$ for any positive integer m .

Solution. We know that

$$\begin{aligned} (AB) \cdot (B^{-1} A^{-1}) &= [(AB) B^{-1}] \cdot A^{-1} = [A(BB^{-1})] \cdot A^{-1} \\ &= [AI] \cdot A^{-1} = A \cdot A^{-1} = I \end{aligned}$$

$$\begin{aligned} \text{Also } B^{-1} A^{-1} \cdot (AB) &= B^{-1} [A^{-1} \cdot (AB)] = B^{-1} [(A^{-1} A) \cdot B] \\ &= B^{-1} [I \cdot B] = B^{-1} \cdot B = I \end{aligned}$$

By definition of the inverse of a matrix, $B^{-1} A^{-1}$ is inverse of AB .

$$B^{-1} A^{-1} = (AB)^{-1}$$

$$\begin{aligned} (A^m)^{-1} &= [A \cdot A^{m-1}]^{-1} = (A^{m-1})^{-1} A^{-1} \\ &= (A \cdot A^{m-2})^{-1} \cdot A^{-1} = [(A^{m-2})^{-1} \cdot A^{-1}] \cdot A^{-1} = (A^{m-2})^{-1} (A^{-1})^2 \\ &= [A \cdot A^{m-3}]^{-1} (A^{-1})^2 = [(A^{m-3})^{-1} \cdot A^{-1}] (A^{-1})^2 = (A^{m-3})^{-1} (A^{-1})^3 \\ &= A^{-1} (A^{-1})^{m-1} = (A^{-1})^m \end{aligned}$$

Proved

Proved

Example 22. Prove that the inverse of a matrix is unique.

Solution. We suppose that B and C are two inverse matrices of a given matrix say

$$\text{Then } AB = BA = I \quad B \text{ is inverse of } A$$

$$\text{and } AC = CA = I \quad C \text{ is inverse of } A$$

$$\text{But } C \cdot (AB) = (CA) \cdot B \quad (\text{Associative})$$

$$\Rightarrow C \cdot I = I \cdot B \text{ or } C = B$$

Hence, the inverse of matrix A is unique.

Proved

Example 23. Find A satisfying the Matrix equation.

$$\begin{bmatrix} 2 & 1 \\ 3 & 2 \end{bmatrix} A \begin{bmatrix} -3 & 2 \\ 5 & -3 \end{bmatrix} = \begin{bmatrix} -2 & 4 \\ 3 & -1 \end{bmatrix}$$

$$\text{Solution. } \begin{bmatrix} 2 & 1 \\ 3 & 2 \end{bmatrix} A \begin{bmatrix} -3 & 2 \\ 5 & -3 \end{bmatrix} = \begin{bmatrix} -2 & 4 \\ 3 & -1 \end{bmatrix}$$

Both sides of the equation are pre-multiplied by the inverse of $\begin{bmatrix} 2 & 1 \\ 3 & 2 \end{bmatrix}$ i.e. $\begin{bmatrix} 2 & -1 \\ -3 & 2 \end{bmatrix}$

$$\begin{bmatrix} 2 & -1 \\ -3 & 2 \end{bmatrix} \begin{bmatrix} 2 & 1 \\ 3 & 2 \end{bmatrix} A \begin{bmatrix} -3 & 2 \\ 5 & -3 \end{bmatrix} = \begin{bmatrix} 2 & -1 \\ -3 & 2 \end{bmatrix} \begin{bmatrix} -2 & 4 \\ 3 & -1 \end{bmatrix}$$

$$\begin{bmatrix} 1 & 0 \\ 0 & 1 \end{bmatrix} A \begin{bmatrix} -3 & 2 \\ 5 & -3 \end{bmatrix} = \begin{bmatrix} -7 & 9 \\ 12 & -14 \end{bmatrix}$$

$$A \begin{bmatrix} -3 & 2 \\ 5 & -3 \end{bmatrix} = \begin{bmatrix} -7 & 9 \\ 12 & -14 \end{bmatrix}$$

Again both sides are post-multiplied by the inverse of $\begin{bmatrix} -3 & 2 \\ 5 & -3 \end{bmatrix}$ i.e. $\begin{bmatrix} 3 & 2 \\ 5 & 3 \end{bmatrix}$

$$A \begin{bmatrix} -3 & 2 \\ 5 & -3 \end{bmatrix} \begin{bmatrix} 3 & 2 \\ 5 & 3 \end{bmatrix} = \begin{bmatrix} -7 & 9 \\ 12 & -14 \end{bmatrix} \begin{bmatrix} 3 & 2 \\ 5 & 3 \end{bmatrix}$$

$$A \begin{bmatrix} 1 & 0 \\ 0 & 1 \end{bmatrix} = \begin{bmatrix} 24 & 13 \\ -34 & -18 \end{bmatrix}$$

$$A = \begin{bmatrix} 24 & 13 \\ -34 & -18 \end{bmatrix} \text{ Ans.}$$

Example 24. Given $A = \begin{bmatrix} 1 & 1 & 1 \\ 2 & 4 & 1 \\ 2 & 3 & 1 \end{bmatrix}$, $B = \begin{bmatrix} 2 & 3 \\ 3 & 4 \end{bmatrix}$

Find C such that $B C A = \begin{bmatrix} 1 & 0 & 1 \\ 0 & 1 & 0 \end{bmatrix}$

Solution. $B C A = \begin{bmatrix} 1 & 0 & 1 \\ 0 & 1 & 0 \end{bmatrix}$

$$\begin{bmatrix} 2 & 3 \\ 3 & 4 \end{bmatrix} C \begin{bmatrix} 1 & 1 & 1 \\ 2 & 4 & 1 \\ 2 & 3 & 1 \end{bmatrix} = \begin{bmatrix} 1 & 0 & 1 \\ 0 & 1 & 0 \end{bmatrix}$$

$$C \begin{bmatrix} 1 & 1 & 1 \\ 2 & 4 & 1 \\ 2 & 3 & 1 \end{bmatrix} = \begin{bmatrix} 2 & 3 \\ 3 & 4 \end{bmatrix}^{-1} \begin{bmatrix} 1 & 0 & 1 \\ 0 & 1 & 0 \end{bmatrix}$$

$$C \begin{bmatrix} 1 & 1 & 1 \\ 2 & 4 & 1 \\ 2 & 3 & 1 \end{bmatrix} = - \begin{bmatrix} 4 & -3 \\ -3 & 2 \end{bmatrix} \begin{bmatrix} 1 & 0 & 1 \\ 0 & 1 & 0 \end{bmatrix}$$

$$C \begin{bmatrix} 1 & 1 & 1 \\ 2 & 4 & 1 \\ 2 & 3 & 1 \end{bmatrix} = - \begin{bmatrix} 4 & -3 & 4 \\ -3 & 2 & -3 \end{bmatrix}$$

$$C = - \begin{bmatrix} 4 & -3 & 4 \\ -3 & 2 & -3 \end{bmatrix} \begin{bmatrix} 1 & 1 & 1 \\ 2 & 4 & 1 \\ 2 & 3 & 1 \end{bmatrix}^{-1}$$

$$C = \begin{bmatrix} 4 & -3 & 4 \\ -3 & 2 & -3 \end{bmatrix} \begin{bmatrix} 1 & 2 & -3 \\ 0 & -1 & 1 \\ -2 & -1 & 2 \end{bmatrix}$$

$$C = \begin{bmatrix} -4 & 7 & -7 \\ 3 & -5 & 5 \end{bmatrix} \text{ Ans.}$$